@prefix : <https://w3id.org/OntoGSN/ontology#> .
@prefix gsn: <https://w3id.org/OntoGSN/ontology#> .
@prefix owl: <http://www.w3.org/2002/07/owl#> .
@prefix rdf: <http://www.w3.org/1999/02/22-rdf-syntax-ns#> .
@prefix xml: <http://www.w3.org/XML/1998/namespace> .
@prefix xsd: <http://www.w3.org/2001/XMLSchema#> .
@prefix rdfs: <http://www.w3.org/2000/01/rdf-schema#> .
@prefix skos: <http://www.w3.org/2004/02/skos/core#> .
@prefix swrl: <http://www.w3.org/2003/11/swrl#> .
@prefix swrla: <http://swrl.stanford.edu/ontologies/3.3/swrla.owl#> .
@prefix swrlb: <http://www.w3.org/2003/11/swrlb#> .
@prefix schema: <http://schema.org/> .
@base <https://w3id.org/OntoGSN/ontology#> .

gsn:applicability rdf:type owl:AnnotationProperty ;
                       rdfs:label "applicability"@en ;
                       skos:definition "The applicability section should state under what circumstances the pattern can be applied, making clear the assumptions and principles underlying the pattern to avoid inappropriate application in a mismatched context. This section should record what contextual information is required in order to apply the pattern."@en ;
                       gsn:coreOrExtension "Argument Pattern Extension"@en ;
                       rdfs:domain gsn:Pattern .

gsn:collaboration rdf:type owl:AnnotationProperty ;
                       rdfs:label "collaboration"@en ;
                       skos:definition "The collaboration section should describe how elements of the pattern work together to achieve the desired effect, particularly where there are links that are not readily apparent from the argument structure."@en ;
                       gsn:coreOrExtension "Argument Pattern Extension"@en ;
                       rdfs:domain gsn:Pattern .

gsn:consequences rdf:type owl:AnnotationProperty ;
                      rdfs:label "consequences"@en ;
                      skos:definition "The consequences section should make clear what work remains after the pattern has been applied. This should highlight where further support to the argument is required, and assumptions that need to be discharged."@en ;
                      gsn:coreOrExtension "Argument Pattern Extension"@en ;
                      rdfs:domain gsn:Pattern .

gsn:examples rdf:type owl:AnnotationProperty ;
                  rdfs:label "examples"@en ;
                  skos:definition "It may be useful to provide example illustrations of the application of the pattern, particularly for more abstract patterns. Illustrations should include a typical case and can be supplemented with atypical cases where more than one example is provided."@en ;
                  gsn:coreOrExtension "Argument Pattern Extension"@en ;
                  rdfs:domain gsn:Pattern .

gsn:implementation rdf:type owl:AnnotationProperty ;
                        rdfs:label "implementation"@en ;
                        skos:definition "The implementation section should communicate how the application of the pattern is carried out e.g. the order in which elements should be developed; communicate hints or techniques that may ease successful application; highlight common or recognised pitfalls with the application of the pattern; and record potential misinterpretation of the terms or concepts in the pattern."@en ;
                        gsn:coreOrExtension "Argument Pattern Extension"@en ;
                        rdfs:domain gsn:Pattern .

gsn:intent rdf:type owl:AnnotationProperty ;
                rdfs:label "intent"@en ;
                skos:definition "The intent statement should state clearly what the pattern aims to achieve."@en ;
                gsn:coreOrExtension "Argument Pattern Extension"@en ;
                rdfs:domain gsn:Pattern .

gsn:knownUses rdf:type owl:AnnotationProperty ;
                   rdfs:label "known uses"@en ;
                   skos:definition "It may be useful to provide references to known applications of the pattern. These can serve as additional examples."@en ;
                   gsn:coreOrExtension "Argument Pattern Extension"@en ;
                   rdfs:domain gsn:Pattern .

gsn:motivation rdf:type owl:AnnotationProperty ;
                    rdfs:label "motivation"@en ;
                    skos:definition "The motivation statement can be used to state why the pattern was created. It could be expressed in terms of previous experiences e.g. as the abstraction of a successfully presented argument, or challenges addressed e.g. argument topics that are often incompletely or poorly addressed."@en ;
                    gsn:coreOrExtension "Argument Pattern Extension"@en ;
                    rdfs:domain gsn:Pattern .

gsn:participants rdf:type owl:AnnotationProperty ;
                      rdfs:label "participants"@en ;
                      skos:definition "The participants section augments the structure by providing a description of each element. This can provide more complete descriptions, clarify the role of the element in the overall argument and emphasise the aspects that require development or instantiation."@en ;
                      gsn:coreOrExtension "Argument Pattern Extension"@en ;
                      rdfs:domain gsn:Pattern .

gsn:structure rdf:type owl:AnnotationProperty ;
                   rdfs:label "structure"@en ;
                   skos:definition "The structure uses the structural and element abstraction notations to present the pattern, clearly indicating where the argument needs to be further developed or populated with details to instantiate the pattern for a specific case."@en ;
                   gsn:coreOrExtension "Argument Pattern Extension"@en ;
                   rdfs:domain gsn:Pattern .

gsn:attachedTo rdf:type owl:ObjectProperty ;
                    rdfs:domain gsn:InstantiationDataReference ;
                    rdfs:range gsn:Template ;
                    rdfs:label "attached to"@en ;
                    gsn:coreOrExtension "Argument Pattern Extension"@en ;
                    gsn:renderedAs "dotted line" .

gsn:instantiationOf rdf:type owl:ObjectProperty ;
                         rdfs:domain [ rdf:type owl:Class ;
                                       owl:unionOf ( gsn:Argument
                                                     gsn:GSNElement
                                                   )
                                     ] ;
                         rdfs:range gsn:Pattern ;
                         rdfs:label "instantiation of"@en ;
                         gsn:coreOrExtension "Argument Pattern Extension"@en .

gsn:relatedTo rdf:type owl:ObjectProperty ;
                   rdfs:domain gsn:Pattern ;
                   rdfs:range gsn:Pattern ;
                   rdfs:label "related to"@en ;
                   skos:definition "This section can be used to reference patterns that are related e.g. addressing the same intent in a different context."@en ;
                   gsn:coreOrExtension "Argument Pattern Extension"@en .

gsn:choice rdf:type owl:DatatypeProperty ;
                rdfs:domain gsn:Relationship ;
                rdfs:range xsd:boolean ;
                rdfs:label "choice"@en ;
                skos:definition "A GSN choice can be used to denote possible alternatives in satisfying a relationship."@en ;
                gsn:coreOrExtension "Argument Pattern Extension"@en ;
                gsn:renderedAs "solid diamond" .

gsn:final rdf:type owl:DatatypeProperty ;
               rdfs:domain gsn:Argument ;
               rdfs:range xsd:boolean ;
               rdfs:label "final"@en ;
               gsn:coreOrExtension "Argument Pattern Extension"@en .

gsn:maxCardinality rdf:type owl:DatatypeProperty ;
                        rdfs:domain gsn:Relationship ;
                        rdfs:range xsd:nonNegativeInteger ;
                        rdfs:label "maximum cardinality"@en ;
                        gsn:coreOrExtension "Argument Pattern Extension"@en ;
                        gsn:renderedAs "text" .

gsn:minCardinality rdf:type owl:DatatypeProperty ;
                        rdfs:domain gsn:Relationship ;
                        rdfs:range xsd:nonNegativeInteger ;
                        rdfs:label "minimum cardinality"@en ;
                        gsn:coreOrExtension "Argument Pattern Extension"@en ;
                        gsn:renderedAs "text" .

gsn:multiple rdf:type owl:DatatypeProperty ;
                  rdfs:domain gsn:Relationship ;
                  rdfs:range xsd:boolean ;
                  rdfs:label "multiple"@en ;
                  gsn:coreOrExtension "Argument Pattern Extension"@en ;
                  gsn:renderedAs "solid ball" .

gsn:optional rdf:type owl:DatatypeProperty ;
                  rdfs:domain gsn:Relationship ;
                  rdfs:range xsd:boolean ;
                  rdfs:label "optional"@en ;
                  skos:definition "Optional instantiation means that the relationship and the argument below may or may not be instantiated."@en ;
                  gsn:coreOrExtension "Argument Pattern Extension"@en ;
                  gsn:renderedAs "hollow ball"@en .

gsn:published rdf:type owl:DatatypeProperty ;
                   rdfs:domain gsn:Argument ;
                   rdfs:range xsd:boolean ;
                   rdfs:label "published"@en ;
                   gsn:coreOrExtension "Argument Pattern Extension"@en .

gsn:undeveloped rdf:type owl:DatatypeProperty ;
                     rdfs:domain [ rdf:type owl:Class ;
                                   owl:unionOf ( gsn:Goal
                                                 gsn:Strategy
                                               )
                                 ] ;
                     rdfs:range xsd:boolean ;
                     rdfs:label "undeveloped"@en ;
                     skos:definition "Undeveloped element decorator, rendered as a hollow diamond applied to the bottom centre of an element, indicates that a line of argument has not been developed."@en ;
                     gsn:coreOrExtension "Argument Pattern Extension"@en ;
                     gsn:renderedAs "hollow diamond" .

gsn:uninstantiated rdf:type owl:DatatypeProperty ;
                        rdfs:domain gsn:GSNElement ;
                        rdfs:range xsd:boolean ;
                        rdfs:label "uninstantiated"@en ;
                        gsn:coreOrExtension "Argument Pattern Extension"@en ;
                        gsn:renderedAs "hollow triangle" .

gsn:Catalogue rdf:type owl:Class ;
                   rdfs:subClassOf [ rdf:type owl:Restriction ;
                                     owl:onProperty gsn:contains ;
                                     owl:allValuesFrom gsn:Pattern
                                   ] ;
                   rdfs:label "Catalogue"@en ;
                   skos:definition "A pattern catalogue may be created to collate a series of patterns; where such a catalogue is created the structure and format of the definition should be consistent and each patternâ€™s definition should have a unique {pattern identifier}."@en ;
                   gsn:coreOrExtension "Argument Pattern Extension"@en .

gsn:InstantiationDataReference rdf:type owl:Class ;
                                    rdfs:label "Instantiation Data Reference"@en ;
                                    skos:definition "This symbol indicates that the GSN argument below the attached element is to be instantiated as a template argument. It provides a reference to the information used to instantiate the template argument." ;
                                    gsn:coreOrExtension "Argument Pattern Extension"@en ;
                                    gsn:renderedAs "hollow triangle" .

gsn:Pattern rdf:type owl:Class ;
                 rdfs:subClassOf [ rdf:type owl:Restriction ;
                                   owl:onProperty schema:description ;
                                   owl:someValuesFrom rdfs:Literal
                                 ] ;
                 rdfs:label "Pattern"@en ;
                 gsn:coreOrExtension "Argument Pattern Extension"@en .


gsn:Template rdf:type owl:Class ;
                  rdfs:subClassOf gsn:Pattern ;
                  rdfs:label "Template"@en ;
                  skos:definition "A template argument is a special case of a pattern argument. It uses the core GSN and argument pattern extension to construct an argument structure which requires no further development."@en ;
                  gsn:coreOrExtension "Argument Pattern Extension"@en .

gsn:A rdf:type swrl:Variable .
gsn:R rdf:type swrl:Variable .
gsn:B rdf:type swrl:Variable .
<urn:swrl:var#B> rdf:type swrl:Variable .
<urn:swrl:var#C> rdf:type swrl:Variable .
<urn:swrl:var#A> rdf:type swrl:Variable .
gsn:C rdf:type swrl:Variable .
gsn:P rdf:type swrl:Variable .

[ swrla:isRuleEnabled "true"^^xsd:boolean ;
   rdfs:comment "" ;
   gsn:coreOrExtension "Argument Pattern Extension" ;
   rdfs:label "S20" ;
   rdf:type swrl:Imp ;
   swrl:body [ rdf:type swrl:AtomList ;
               rdf:first [ rdf:type swrl:IndividualPropertyAtom ;
                           swrl:propertyPredicate gsn:instantiationOf ;
                           swrl:argument1 gsn:B ;
                           swrl:argument2 gsn:C
                         ] ;
               rdf:rest [ rdf:type swrl:AtomList ;
                          rdf:first [ rdf:type swrl:DatavaluedPropertyAtom ;
                                      swrl:propertyPredicate gsn:final ;
                                      swrl:argument1 gsn:A ;
                                      swrl:argument2 "true"^^xsd:boolean
                                    ] ;
                          rdf:rest [ rdf:type swrl:AtomList ;
                                     rdf:first [ rdf:type swrl:ClassAtom ;
                                                 swrl:classPredicate gsn:Pattern ;
                                                 swrl:argument1 gsn:C
                                               ] ;
                                     rdf:rest [ rdf:type swrl:AtomList ;
                                                rdf:first [ rdf:type swrl:IndividualPropertyAtom ;
                                                            swrl:propertyPredicate gsn:contains ;
                                                            swrl:argument1 gsn:A ;
                                                            swrl:argument2 gsn:B
                                                          ] ;
                                                rdf:rest [ rdf:type swrl:AtomList ;
                                                           rdf:first [ rdf:type swrl:IndividualPropertyAtom ;
                                                                       swrl:propertyPredicate gsn:contains ;
                                                                       swrl:argument1 gsn:A ;
                                                                       swrl:argument2 gsn:C
                                                                     ] ;
                                                           rdf:rest rdf:nil
                                                         ]
                                              ]
                                   ]
                        ]
             ] ;
   swrl:head [ rdf:type swrl:AtomList ;
               rdf:first [ rdf:type swrl:DatavaluedPropertyAtom ;
                           swrl:propertyPredicate gsn:valid ;
                           swrl:argument1 gsn:A ;
                           swrl:argument2 "false"^^xsd:boolean
                         ] ;
               rdf:rest rdf:nil
             ]
 ] .

[ swrla:isRuleEnabled "true"^^xsd:boolean ;
   rdfs:comment "" ;
   gsn:coreOrExtension "Argument Pattern Extension" ;
   rdfs:label "S21" ;
   rdf:type swrl:Imp ;
   swrl:body [ rdf:type swrl:AtomList ;
               rdf:first [ rdf:type swrl:ClassAtom ;
                           swrl:classPredicate gsn:Template ;
                           swrl:argument1 gsn:A
                         ] ;
               rdf:rest [ rdf:type swrl:AtomList ;
                          rdf:first [ rdf:type swrl:DatavaluedPropertyAtom ;
                                      swrl:propertyPredicate gsn:undeveloped ;
                                      swrl:argument1 gsn:R ;
                                      swrl:argument2 "true"^^xsd:boolean
                                    ] ;
                          rdf:rest [ rdf:type swrl:AtomList ;
                                     rdf:first [ rdf:type swrl:IndividualPropertyAtom ;
                                                 swrl:propertyPredicate rdf:subject ;
                                                 swrl:argument1 gsn:R ;
                                                 swrl:argument2 gsn:A
                                               ] ;
                                     rdf:rest [ rdf:type swrl:AtomList ;
                                                rdf:first [ rdf:type swrl:DatavaluedPropertyAtom ;
                                                            swrl:propertyPredicate gsn:published ;
                                                            swrl:argument1 gsn:A ;
                                                            swrl:argument2 "true"^^xsd:boolean
                                                          ] ;
                                                rdf:rest rdf:nil
                                              ]
                                   ]
                        ]
             ] ;
   swrl:head [ rdf:type swrl:AtomList ;
               rdf:first [ rdf:type swrl:DatavaluedPropertyAtom ;
                           swrl:propertyPredicate gsn:valid ;
                           swrl:argument1 gsn:A ;
                           swrl:argument2 "false"^^xsd:boolean
                         ] ;
               rdf:rest [ rdf:type swrl:AtomList ;
                          rdf:first [ rdf:type swrl:DatavaluedPropertyAtom ;
                                      swrl:propertyPredicate gsn:valid ;
                                      swrl:argument1 gsn:R ;
                                      swrl:argument2 "false"^^xsd:boolean
                                    ] ;
                          rdf:rest rdf:nil
                        ]
             ]
 ] .

[ swrla:isRuleEnabled "true"^^xsd:boolean ;
   rdfs:comment "" ;
   gsn:coreOrExtension "Argument Pattern Extension" ;
   rdfs:label "S22" ;
   rdf:type swrl:Imp ;
   swrl:body [ rdf:type swrl:AtomList ;
               rdf:first [ rdf:type swrl:ClassAtom ;
                           swrl:classPredicate gsn:Template ;
                           swrl:argument1 gsn:A
                         ] ;
               rdf:rest [ rdf:type swrl:AtomList ;
                          rdf:first [ rdf:type swrl:DatavaluedPropertyAtom ;
                                      swrl:propertyPredicate gsn:undeveloped ;
                                      swrl:argument1 gsn:R ;
                                      swrl:argument2 "true"^^xsd:boolean
                                    ] ;
                          rdf:rest [ rdf:type swrl:AtomList ;
                                     rdf:first [ rdf:type swrl:IndividualPropertyAtom ;
                                                 swrl:propertyPredicate rdf:subject ;
                                                 swrl:argument1 gsn:R ;
                                                 swrl:argument2 gsn:B
                                               ] ;
                                     rdf:rest [ rdf:type swrl:AtomList ;
                                                rdf:first [ rdf:type swrl:DatavaluedPropertyAtom ;
                                                            swrl:propertyPredicate gsn:published ;
                                                            swrl:argument1 gsn:A ;
                                                            swrl:argument2 "true"^^xsd:boolean
                                                          ] ;
                                                rdf:rest [ rdf:type swrl:AtomList ;
                                                           rdf:first [ rdf:type swrl:IndividualPropertyAtom ;
                                                                       swrl:propertyPredicate gsn:contains ;
                                                                       swrl:argument1 gsn:A ;
                                                                       swrl:argument2 gsn:B
                                                                     ] ;
                                                           rdf:rest rdf:nil
                                                         ]
                                              ]
                                   ]
                        ]
             ] ;
   swrl:head [ rdf:type swrl:AtomList ;
               rdf:first [ rdf:type swrl:DatavaluedPropertyAtom ;
                           swrl:propertyPredicate gsn:valid ;
                           swrl:argument1 gsn:A ;
                           swrl:argument2 "false"^^xsd:boolean
                         ] ;
               rdf:rest [ rdf:type swrl:AtomList ;
                          rdf:first [ rdf:type swrl:DatavaluedPropertyAtom ;
                                      swrl:propertyPredicate gsn:valid ;
                                      swrl:argument1 gsn:R ;
                                      swrl:argument2 "false"^^xsd:boolean
                                    ] ;
                          rdf:rest rdf:nil
                        ]
             ]
 ] .